Added relational Hoare logic, refinement calculus, and wlp

ITree_Relation.thy
@@ -16,6 +16,36 @@ text \<open> The precondition captures the initial states that give the possibil
 definition itree_pre :: "('e, 's) htree \<Rightarrow> ('s \<Rightarrow> bool)" where
 "itree_pre P = (\<lambda> s. \<not> (\<exists> es. P s \<midarrow>es\<leadsto> diverge))"
 
+expr_ctr itree_pre
+
+definition refined_by :: "('e, 's) htree \<Rightarrow> ('e, 's) htree \<Rightarrow> bool" (infix "\<sqsubseteq>" 50) where
+"refined_by P Q = (`itree_pre P \<longrightarrow> itree_pre Q` \<and> {(s, s') \<in> itree_rel Q. itree_pre P s} \<subseteq> itree_rel P)"
+
+definition spec :: "'s scene \<Rightarrow> ('s \<Rightarrow> bool) \<Rightarrow> ('s \<Rightarrow> bool) \<Rightarrow> 's rel" where
+"spec a pre post = {(s, s'). s \<approx>\<^sub>S s' on (- a) \<and> pre s \<longrightarrow> post s'}"
+
+definition hoare_triple :: "('s \<Rightarrow> bool) \<Rightarrow> ('e, 's) htree \<Rightarrow> ('s \<Rightarrow> bool) \<Rightarrow> bool" where
+"hoare_triple P S Q = (itree_rel S \<subseteq> spec \<top>\<^sub>S P Q)"
+
+syntax "_hoare" :: "logic \<Rightarrow> logic \<Rightarrow> logic \<Rightarrow> logic" ("\<^bold>{_\<^bold>} _ \<^bold>{_\<^bold>}")
+translations "_hoare P S Q" == "CONST hoare_triple (P)\<^sub>e S (Q)\<^sub>e"
+
+lemma hoare_alt_def: "\<^bold>{P\<^bold>} S \<^bold>{Q\<^bold>} \<longleftrightarrow> (\<forall> s s' es. P s \<and> S s \<midarrow>es\<leadsto> Ret s' \<longrightarrow> Q s')"
+  by (auto simp add: hoare_triple_def spec_def itree_rel_def retvals_def subset_iff)
+
+named_theorems wp
+
+definition wlp_itree :: "('e, 's) htree \<Rightarrow> ('s \<Rightarrow> bool) \<Rightarrow> ('s \<Rightarrow> bool)" where
+"wlp_itree S P = (\<lambda>s. \<forall>s'. (s, s') \<in> itree_rel S \<longrightarrow> P s')"
+
+expr_ctr wlp_itree
+
+syntax "_wlp" :: "logic \<Rightarrow> logic \<Rightarrow> logic" ("wlp")
+translations "_wlp S P" == "CONST wlp_itree S (P)\<^sub>e"
+
+lemma wlp_true [wp]: "wlp P True = (True)\<^sub>e"
+  by (expr_simp add: wlp_itree_def)
+  
 lemma assigns_rel: "itree_rel \<langle>\<sigma>\<rangle>\<^sub>a = {(s, s'). s' = \<sigma> s}"
   by (auto simp add: itree_rel_def retvals_def assigns_def)
 
@@ -28,11 +58,25 @@ lemma Div_rel: "itree_rel Div = {}"
 lemma Div_pre: "itree_pre Div = (False)\<^sub>e"
   by (auto simp add: itree_pre_def fun_eq_iff)
 
+lemma Div_wlp: "wlp Div P = (True)\<^sub>e"
+  by (simp add: wlp_itree_def Div_rel, expr_simp)
+
+
+lemma Div_bottom: "Div \<sqsubseteq> P"
+  by (simp add: refined_by_def Div_rel Div_pre)
+
 lemma Stop_rel: "itree_rel Stop = {}"
   by (simp add: itree_rel_def)
 
 lemma Stop_pre: "itree_pre Stop = (True)\<^sub>e"
   by (auto simp add: itree_pre_def fun_eq_iff deadlock_def)
+
+lemma seq_pre: "itree_pre (P \<Zcomp> Q) = (itree_pre P \<and> wlp P (itree_pre Q))\<^sub>e"
+  apply (expr_simp, auto elim!: trace_to_bindE simp add: itree_pre_def wlp_itree_def itree_rel_def retvals_def)
+  apply (metis bind_diverge trace_to_bind_left)
+  apply (meson trace_to_bind)
+  apply (metis trace_of_Sils trace_to_Nil trace_to_trans)
+  done
 
 lemma seq_rel: "itree_rel (P \<Zcomp> Q) = itree_rel P O itree_rel Q"
   by (auto simp add: itree_rel_def relcomp_unfold)
@@ -45,11 +89,5 @@ lemma input_rel: "wb_prism c \<Longrightarrow> itree_rel (input c P) = (\<Union>
 
 lemma input_in_lit_rel: "wb_prism c \<Longrightarrow> itree_rel (input_in c (\<guillemotleft>A\<guillemotright>)\<^sub>e P) = (\<Union> v \<in> A. itree_rel (P v))"
   by (auto simp add: input_in_rel input_alt_def)
-
-definition spec :: "'s scene \<Rightarrow> ('s \<Rightarrow> bool) \<Rightarrow> ('s \<Rightarrow> bool) \<Rightarrow> 's rel" where
-"spec a pre post = {(s, s'). s \<approx>\<^sub>S s' on (- a) \<and> pre s \<longrightarrow> post s'}"
-
-definition hoare_triple :: "('s \<Rightarrow> bool) \<Rightarrow> ('e, 's) htree \<Rightarrow> ('s \<Rightarrow> bool) \<Rightarrow> bool" where
-"hoare_triple P S Q = (spec \<top>\<^sub>S P Q \<subseteq> itree_rel S)"
 
 end
